src/lowparse/LowParse.Low.Int.fsti
@@ -43,68 +43,14 @@ inline_for_extraction
 let validate_nochk32_u32 : validator_nochk32 parse_u32 =
   validate_nochk32_constant_size parse_u32 4ul ()
 
-val serialize32_u16
-  (b: buffer8)
-  (lo: U32.t)
-  (v: U16.t)
-: HST.Stack unit
-  (requires (fun h -> B.live h b /\ U32.v lo + 2 <= B.length b))
-  (ensures (fun h _ h' ->
-    M.modifies (M.loc_buffer (B.gsub b lo (2ul))) h h' /\
-    B.live h' b /\
-    exactly_contains_valid_data h' parse_u16 b lo v (U32.add lo 2ul)
-  ))
+inline_for_extraction
+val serialize32_u16 : serializer32 serialize_u16
 
-val serialize32_u32
-  (b: buffer8)
-  (lo: U32.t)
-  (v: U32.t)
-: HST.Stack unit
-  (requires (fun h -> B.live h b /\ U32.v lo + 4 <= B.length b))
-  (ensures (fun h _ h' ->
-    M.modifies (M.loc_buffer (B.gsub b lo (4ul))) h h' /\
-    B.live h' b /\
-    exactly_contains_valid_data h' parse_u32 b lo v (U32.add lo 4ul)
-  ))
+inline_for_extraction
+val serialize32_u32 : serializer32 serialize_u32
 
-module Cast = FStar.Int.Cast
+inline_for_extraction
+val serialize32_u16_fail : serializer32_fail serialize_u16
 
-val serialize32_u16_fail
-  (b: buffer8)
-  (len: I32.t { I32.v len == B.length b } )
-  (lo: I32.t)
-  (v: U16.t)
-: HST.Stack I32.t
-  (requires (fun h -> B.live h b))
-  (ensures (fun h hi h' ->
-    B.live h' b /\
-    contains_valid_serialized_data_or_fail h' serialize_u16 b lo v hi /\
-    M.modifies (
-      if I32.v lo < 0
-      then M.loc_none
-      else if I32.v hi < 0
-      then M.loc_buffer (B.gsub b (Cast.int32_to_uint32 lo) (B.len b `U32.sub` Cast.int32_to_uint32 lo))
-      else M.loc_buffer (B.gsub b (Cast.int32_to_uint32 lo) (Cast.int32_to_uint32 (hi `I32.sub` lo)))
-    )
-    h h'
-  ))
-
-val serialize32_u32_fail
-  (b: buffer8)
-  (len: I32.t { I32.v len == B.length b } )
-  (lo: I32.t)
-  (v: U32.t)
-: HST.Stack I32.t
-  (requires (fun h -> B.live h b))
-  (ensures (fun h hi h' ->
-    B.live h' b /\
-    contains_valid_serialized_data_or_fail h' serialize_u32 b lo v hi /\
-    M.modifies (
-      if I32.v lo < 0
-      then M.loc_none
-      else if I32.v hi < 0
-      then M.loc_buffer (B.gsub b (Cast.int32_to_uint32 lo) (B.len b `U32.sub` Cast.int32_to_uint32 lo))
-      else M.loc_buffer (B.gsub b (Cast.int32_to_uint32 lo) (Cast.int32_to_uint32 (hi `I32.sub` lo)))
-    )
-    h h'
-  ))
+inline_for_extraction
+val serialize32_u32_fail : serializer32_fail serialize_u32
